Heap/Delete.v
@@ -1,6 +1,7 @@
 Require Import Coq.Lists.List.
 Require Import Coq.ZArith.ZArith.
 Require Import Coq.Classes.RelationClasses.
+Require Import Coq.micromega.Psatz.
 Require Import PL.Monad.
 Require Import PL.Monad2.
 Require Import SetsClass.
@@ -24,21 +25,98 @@ Local Open Scope monad.
 4. 保持满二叉树 *)
 
 Theorem ext_delete_node_correctness1: forall (val: Z) (V: Z -> Prop),
-  Hoare (fun s => ((exists lc: Z, BinaryTree.step_l s.(heap) val lc) \/
-                        (exists rc: Z, BinaryTree.step_r s.(heap) val rc)) /\
-                  Abs s.(heap) V /\
-                  BinaryTree.legal s.(heap) /\
-                  Heap s.(heap) /\ 
-                  s.(heap).(vvalid) val)
+  Hoare (fun s => (exists lc : Z, BinaryTree.step_l s.(heap) val lc \/
+                    (exists rc : Z, BinaryTree.step_r s.(heap) val rc)) /\
+                  Abs s.(heap) V /\ 
+                  BinaryTree.legal s.(heap) /\ 
+                  Heap s.(heap) /\
+                  is_minimum val V)
         (ext_delete_node val)
+        (fun v s => s.(heap).(vvalid) v /\
+                    (s.(heap).(vvalid) ∪ Sets.singleton val) == V /\
+                    is_minimum val V /\
+                    BinaryTree.legal s.(heap) /\
+                    (Heap_broken_down s.(heap) v \/ Heap s.(heap))).
+Proof.
+  intros.
+  unfold ext_delete_node.
+  unfold Hoare, Abs; sets_unfold.
+  intros.
+  destruct H as [? [? [? [? ?]]]].
+  destruct H0 as [? [? [? [? [? ?]]]]].
+  - split; [tauto| split; [| split; [| split]]].
+    + intros.
+      rewrite H1.
+      apply H6.
+    + tauto.
+    + tauto.
+    + tauto.
+Qed.
+
+Theorem ext_delete_node_correctness2: forall (val: Z),
+  Hoare (fun s => (exists lc : Z, BinaryTree.step_l s.(heap) val lc \/
+                    (exists rc : Z, BinaryTree.step_r s.(heap) val rc)) /\
+                  is_complete_or_full_bintree s.(heap))
+        (ext_delete_node val)
+        (fun v s => is_complete_or_full_bintree s.(heap)).
+Proof.
+  intros.
+  unfold ext_delete_node.
+  unfold Hoare, Abs; sets_unfold.
+  intros.
+  destruct H as [? ?].
+  destruct H0 as [? [? [? ?]]].
+  tauto.
+Qed.
+
+
+Theorem delete_iso_node_correctness1: forall (val: Z) (V: Z -> Prop),
+  Hoare (fun s: state =>
+                        ((s.(heap)).(vvalid) val /\
+                        ~ (exists lc : Z, BinaryTree.step_l s.(heap) val lc) /\
+                        ~ (exists rc : Z, BinaryTree.step_r s.(heap) val rc)) /\
+                        Abs s.(heap) V /\ 
+                        BinaryTree.legal s.(heap) /\ 
+                        Heap s.(heap) /\
+                        is_minimum val V)
+        (ext_delete_iso_node val)
         (fun _ s => (s.(heap).(vvalid) ∪ Sets.singleton val) == V /\
                     is_minimum val V /\
                     BinaryTree.legal s.(heap) /\
-                    (Heap_broken_down s.(heap) val \/ Heap s.(heap))).
-Admitted.
+                    Heap s.(heap)).
+Proof.
+  intros.
+  unfold ext_delete_iso_node.
+  unfold Hoare, Abs; sets_unfold.
+  intros.
+  destruct H as [[? [? ?]] [? [? [? ?]]]].
+  destruct H0 as [? [? [? ?]]].
+  split; [| split; [| split]].
+  - intros.
+    rewrite H3.
+    apply H7.
+  - tauto.
+  - tauto.
+  - tauto.
+Qed.
 
-(* Theorem delete_iso_node_correctness1 *)
-
+Theorem delete_iso_node_correctness2: forall (val: Z),
+  Hoare (fun s: state =>
+                        ((s.(heap)).(vvalid) val /\
+                        ~ (exists lc : Z, BinaryTree.step_l s.(heap) val lc) /\
+                        ~ (exists rc : Z, BinaryTree.step_r s.(heap) val rc)) /\
+                        is_complete_or_full_bintree s.(heap))
+        (ext_delete_iso_node val)
+        (fun _ s => is_complete_or_full_bintree s.(heap)).
+Proof.
+  intros.
+  unfold ext_delete_iso_node.
+  unfold Hoare, Abs; sets_unfold.
+  intros.
+  destruct H as [? ?].
+  destruct H0 as [? [? [? ?]]].
+  tauto.
+Qed.
 
 (* 删除操作正确性（保证非空的前提下（似乎没用））：
 1. 删除的元素是最小值
@@ -57,15 +135,54 @@ Theorem delete_correctness1: forall (V: Z -> Prop), ~ V == ∅ ->
 Proof.
   intros.
   unfold delete.
-  eapply Hoare_bind; [apply get_minimum_correctness| cbv beta].
-  intros v.
+  eapply Hoare_bind; [apply get_min_correctness1| cbv beta].
+  intros val.
   apply Hoare_choice.
   - apply Hoare_test_bind.
-    (* eapply Hoare_bind; [apply delete_iso_node_correctness1| cbv beta]. *)
-    admit.
+    eapply Hoare_bind; [apply delete_iso_node_correctness1| cbv beta].
+    intros.
+    apply Hoare_ret'.
+    intros.
+    destruct H0 as [? [? [? ?]]].
+    split; [| split; [tauto | tauto]].
+    tauto.
   - apply Hoare_test_bind.
-    revert v.
-    (* eapply Hoare_bind; [apply ext_delete_node_correctness1| cbv beta].
-     *)
-    
-Admitted.
+    revert val.
+    intros.
+    eapply Hoare_bind; [apply ext_delete_node_correctness1| cbv beta].
+    intros v.
+    eapply Hoare_bind; [apply move_down_helper1| cbv beta].
+    intros.
+    apply Hoare_ret'.
+    intros.
+    destruct H0 as [? [? [? ?]]].
+    split; [| split; [tauto | tauto]].
+    tauto.
+Qed.
+
+Theorem delete_correctness2: forall (V: Z -> Prop),
+  Hoare (fun s => is_complete_or_full_bintree s.(heap))
+        delete
+        (fun _ s => is_complete_or_full_bintree s.(heap)).
+Proof.
+  intros.
+  unfold delete.
+  eapply Hoare_bind; [apply get_min_correctness2| cbv beta].
+  intros val.
+  apply Hoare_choice.
+  - apply Hoare_test_bind.
+    eapply Hoare_bind; [apply delete_iso_node_correctness2| cbv beta].
+    intros.
+    apply Hoare_ret'.
+    intros.
+    tauto.
+  - apply Hoare_test_bind.
+    eapply Hoare_bind; [apply ext_delete_node_correctness2| cbv beta].
+    intros v.
+    eapply Hoare_bind; [apply move_down_correctness2| cbv beta].
+    intros.
+    apply Hoare_ret'.
+    intros.
+    tauto.
+Qed.
+  
